\subsection{Quantifier Ambiguity}

Sentences such as ``Every man loves a woman'' or ``Every owner of a siamese
cat loves a therapist'' are ambiguous. In ACGs, every abstract derivation
has exactly one object interpretation. In order to account for ambiguity,
we have two ways of proceeding. Either we introduce separate derivations to
account for the different readings or we make our interpretations
non-deterministic, underspecified. In the next two subsections, we will
explore both techniques.

\subsubsection{QR}

We propose a small extension which adds the $\abs{QR}$ operator to our
fragment. The goal of this operator is to let us project the effects
(e.g.\ scope-taking) of any $NP$ outside of its ``usual'' destination.

We give an update to the abstract signature, $\Sigma^a_{QR}$:

\begin{align*}
  \abs{QR} &: NP \to (NP \to S) \to S
\end{align*}

And we give a semantics to the $\abs{QR}$ operator in $\mathcal{L}_{QR}$:

\begin{align*}
  \lex{QR}{\lambda X k.\ \mathrm{SI}\ (X \hsbind (\lambda x.\ k\ (\eta\ x)))}
\end{align*}

Now, the extension is complete.

$$
E_{QR}(\left< \Sigma^a, \Sigma^o, \mathcal{L} \right>) = \left< \Sigma^a \uplus \Sigma^a_{QR}, \Sigma^o, \mathcal{L} \uplus \mathcal{L}_{QR} \right>
$$

We can now derive the inverse scope reading of ``Every man loves a woman''.

\begin{align*}
& \sem{\abs{QR}\ (\abs{a}\ \abs{woman})\ (\lambda
    x.\ \abs{loves}\ x\ (\abs{every}\ \abs{man}))} \\
\rightarrow^*\ & \mathrm{SI}\ (SCOPE\ (\lambda k.\ \dexists
x.\ (\eta\ (\obj{woman}\ x)) \dand (k\ x))\ (\lambda x.\ \eta\ (\forall
y.\ \obj{man}\ y \rightarrow \obj{love}\ y\ x))) \\
\rightarrow^*\ & (\lambda k.\ \dexists
x.\ (\eta\ (\obj{woman}\ x)) \dand (k\ x))\ (\lambda x.\ \eta\ (\forall
y.\ \obj{man}\ y \rightarrow \obj{love}\ y\ x)) \\
\rightarrow^*\ & \eta\ (\exists x.\ \obj{woman}\ x \land (\forall
y.\ \obj{man}\ y \rightarrow \obj{love}\ y\ x))
\end{align*}

The QR operator allows us to displace the scope of any quantifier
(actually, it can displace any kind of $NP$ effect, including dynamics, so
it can be used, e.g., to implement a kind of cataphora).

\subsubsection{Leaky Scope Islands}

We will now look at a solution that over-generates a little less and that
is based on a different strategy. Rather than having different derivations
that place the quantifier scope at different locations, we will weaken the
scope islands so that they may choose to let a quantifier escape.

In order to allow for choice and non-determinism, we will add a new effect,
$CHOOSE : 1 \to 2 \in E$, where $2$ is the Boolean type $1 +
1$\footnote{For this to work, we assume the presence of standard sum types
  (intuitionistic disjunction on types) in our calculus.}. We will also
introduce the following syntactic sugar for non-deterministic computations:

\begin{align*}
A + B = CHOOSE\ *\ (\lambda b.\ \text{case}\ b\ \text{of}\ &\operatorname{inl}(*) \Rightarrow A \\
|\ &\operatorname{inr}(*) \Rightarrow B)
\end{align*}

We would like certain quantifiers (e.g., indefinites) to be able to escape
scope islands. We will introduce an effect $SCOPE_P : ((\iota \to
\mathcal{F}(o)) \to \mathcal{F}(o)) \to \iota \in E$, which is a variant of
the $SCOPE$ effect to be used by quantifiers that ought to be able to
escape from scope islands.

We can now define our extension $E_{Q'}$, which builds upon $E_Q$:

$$
E_{Q'}(\left< \Sigma^a, \Sigma^o, \mathcal{L} \right>) =
\left< \Sigma^a, \Sigma^o, \mathcal{L} \uplus \mathcal{L}_{Q'} \right>
$$

where, $\mathcal{L}_{Q'}$, the changes we propose to the lexicon, are as
follows:

\begin{align*}
  \lex{every}{\lambda N.\ SCOPE\ (\lambda k.\ \mathrm{SL}\ (\dforall\ (\lambda x.\ (N \apl x) \dimp (k\ x))))}\ \eta \\
  \sem{\abs{some}} := \sem{\abs{a}} &:= \lambda N.\ SCOPE_P\ (\lambda k.\ \mathrm{SL}\ (\dexists\ (\lambda x.\ (N \apl x) \dand (k\ x))))\ \eta \\
  \mathrm{SI} &= \mathcal{L}(\mathrm{SI}) \circ \mathrm{SL} \\
  \mathrm{SL} &: \mathcal{F}(o) \to \mathcal{F}(o) \\
  \mathrm{SL} &= [\mathcal{H}\ (SCOPE_P\ (\lambda c k.\ (c\ k) + (SCOPE_P\ c\ k)))] 
\end{align*}

The $\mathrm{SL}$ (Scope Location) handler introduces a possible place for
a quantifier to take scope.

We will now look again at the sentence ``Every man loves a woman''. First
off, we will introduce some handy shortcuts:

\begin{align*}
c_1 &= \lambda k. \dforall\ (\lambda x.\ (\eta\ (\obj{man}\ x)) \dimp (k\ x)) \\
c_2 &= \lambda k.\ \dexists\ (\lambda x.\ (\eta\ (\obj{woman}\ x)) \dand
(k\ x)) \\
\sem{\abs{every}\ \abs{man}} &= SCOPE\ (\mathrm{SL} \circ c_1)\ \eta \\
\sem{\abs{a}\ \abs{woman}} &= SCOPE_P\ (\mathrm{SL} \circ c_2)\ \eta
\end{align*}


\begin{align*}
  & \sem{\abs{loves}\ (\abs{a}\ \abs{woman})\ (\abs{every}\ \abs{man})} \\
  \rightarrow^*\ & \mathrm{SI}\ (SCOPE\ (\mathrm{SL} \circ c_1)\ 
  (\lambda x.\ SCOPE_P\ (\mathrm{SL} \circ c_2)\
  (\lambda y.\ \eta\ (\obj{love}\ x\ y)))) \\
  \rightarrow^*\ & \mathrm{SL}\ (c_1\
  (\lambda x.\ \mathrm{SI}\ (SCOPE_P\ (\mathrm{SL} \circ c_2)\
  (\lambda y.\ \eta\ (\obj{love}\ x\ y))))) \\
  \rightarrow^*\ & \mathrm{SL}\ (c_1\
  (\lambda x.\ \mathrm{SL}\ (c_2\ 
  (\lambda y.\ \mathrm{SI}\ (\eta\ (\obj{love}\ x\ y)))) +
  SCOPE_P\ (\mathrm{SL} \circ c_2)\
  (\lambda y.\ \mathrm{SI}\ (\eta\ (\obj{love}\ x\ y))))) \\
  \rightarrow^*\ & \mathrm{SL}\ (c_1\
  (\lambda x.\ \mathrm{SL}\ (c_2\ 
  (\lambda y.\ \eta\ (\obj{love}\ x\ y))) +
  SCOPE_P\ (\mathrm{SL} \circ c_2)\
  (\lambda y.\ \eta\ (\obj{love}\ x\ y)))) \\
  \rightarrow^*\ & \mathrm{SL}\ (c_1\ (\lambda x.\ 
  \mathrm{SL}\ (\eta\ (\exists y.\ \obj{woman}\ y \land \obj{love}\ x\ y) +
  SCOPE_P\ (\mathrm{SL} \circ c_2)\
  (\lambda y.\ \eta\ (\obj{love}\ x\ y)))) \\
  \rightarrow^*\ & \mathrm{SL}\ (c_1\ (\lambda x.\ 
  (\eta\ (\exists y.\ \obj{woman}\ y \land \obj{love}\ x\ y) +
  SCOPE_P\ (\mathrm{SL} \circ c_2)\
  (\lambda y.\ \eta\ (\obj{love}\ x\ y)))) \\
  \rightarrow^*\ & \mathrm{SL}\ (\eta\ (\forall x.\ \obj{man}\ x
  \rightarrow (\exists y.\ \obj{woman}\ y \land \obj{love}\ x\ y)) \\
  & \hspace{7mm} + SCOPE_P\ (\mathrm{SL} \circ c_2)\ (\lambda y.\ 
  \eta\ (\forall x.\ \obj{man}\ x \rightarrow \obj{love}\ x\ y))) \\
  \rightarrow^*\ & \mathrm{SL}\ (\eta\ (\forall x.\ \obj{man}\ x
  \rightarrow (\exists y.\ \obj{woman}\ y \land \obj{love}\ x\ y))) \\
  +\ & \mathrm{SL}\ (SCOPE_P\ (\mathrm{SL} \circ c_2)\ (\lambda y.\
  \eta\ (\forall x.\ \obj{man}\ x \rightarrow \obj{love}\ x\ y))) \\
  \rightarrow^*\ & \eta\ (\forall x.\ \obj{man}\ x
  \rightarrow (\exists y.\ \obj{woman}\ y \land \obj{love}\ x\ y)) \\
  +\ & \mathrm{SL}\ (c_2\ (\lambda y.\ \eta\ (\forall x.\
  \obj{man}\ x \rightarrow \obj{love}\ x\ y))) \\
  +\ & SCOPE_P\ (\mathrm{SL} \circ c_2)\ (\lambda y.\ \eta\ (\forall x.\
  \obj{man}\ x \rightarrow \obj{love}\ x\ y))) \\
  \rightarrow^*\ & \eta\ (\forall x.\ \obj{man}\ x
  \rightarrow (\exists y.\ \obj{woman}\ y \land \obj{love}\ x\ y)) \\
  +\ & \mathrm{SL}\ (\eta\ (\exists y.\ \obj{woman}\ y \land (\forall x.\
  \obj{man}\ x \rightarrow \obj{love}\ x\ y))) \\
  +\ & SCOPE_P\ (\mathrm{SL} \circ c_2)\ (\lambda y.\ \eta\ (\forall x.\
  \obj{man}\ x \rightarrow \obj{love}\ x\ y)) \\
  \rightarrow^*\ & \eta\ (\forall x.\ \obj{man}\ x
  \rightarrow (\exists y.\ \obj{woman}\ y \land \obj{love}\ x\ y)) \\
  +\ & \eta\ (\exists y.\ \obj{woman}\ y \land (\forall x.\
  \obj{man}\ x \rightarrow \obj{love}\ x\ y)) \\
  +\ & SCOPE_P\ (\mathrm{SL} \circ c_2)\ (\lambda y.\ \eta\ (\forall x.\
  \obj{man}\ x \rightarrow \obj{love}\ x\ y)) \\
\end{align*}

\begin{align*}
  & \sem{\abs{who}\ (\abs{knows}\ (\abs{a}\ \abs{cat}))\ \abs{man}} \\
  \rightarrow^*\ & \mathcal{C}\ (\lambda x.\ (\eta\ (\obj{man}\ x)) \dand
  \sem{\abs{knows}\ (\abs{a}\ \abs{cat})\ (\eta\ x)}) \\
  \rightarrow^*\ & \mathcal{C}\ (\lambda x.\ (\eta\ (\obj{man}\ x)) \dand
  (\mathrm{SI}\ (SCOPE_P\ c_{cat}\ (\lambda y.\ \eta\ (\obj{know}\ x\ y))))) \\
  \rightarrow^*\ & \mathcal{C}\ (\lambda x.\ (\eta\ (\obj{man}\ x)) \dand
  ((c_{cat}\ (\lambda y.\ \eta\ (\obj{know}\ x\ y))) +
  (SCOPE_P\ c_{cat}\ (\lambda y.\ \eta\ (\obj{know}\ x\ y)))) \\
  \rightarrow^*\ & \mathcal{C}\ (\lambda x.\ (\eta\ (\obj{man}\ x)) \dand
  ((\eta\ (\exists y.\ (\obj{cat}\ y \land \obj{know}\ x\ y))) +
  (SCOPE_P\ c_{cat}\ (\lambda y.\ \eta\ (\obj{know}\ x\ y)))) \\
  \rightarrow^*\ & \eta\ (\lambda x.\ \obj{man}\ x \land
  (\exists y.\ \obj{cat}\ y \land \obj{know}\ x\ y)) \\
  +\ & SCOPE_P\ c_{cat}\ (\lambda y.\ \eta\ (\lambda x.\ (\obj{man}\ x \land \obj{know}\ x\ y))) \\
\end{align*}

\begin{align*}
  & \sem{\abs{every}\ (\abs{who}\ (\abs{knows}\ (\abs{a}\ \abs{cat}))\ \abs{man})} \\
\rightarrow^*\ & SCOPE\ (\lambda k.\ \mathrm{SL}\ ((\dforall x.\
  \eta\ (\obj{man}\ x \land (\exists y.\ \obj{cat}\ y \land
  \obj{know}\ x\ y)) \dimp (k\ x))) \\
  & \hspace{25mm} + SCOPE_P\ c_{cat}\ (\lambda y.\ \dforall x.\ (\eta\ (\obj{man}\ x
  \land \obj{know}\ x\ y)) \dimp (k\ x)))\ \eta \\
\rightarrow^*\ & SCOPE\ (\lambda k.\ (\mathrm{SL}\ (\dforall x.\
  \eta\ (\obj{man}\ x \land (\exists y.\ \obj{cat}\ y \land
  \obj{know}\ x\ y)) \dimp (k\ x))) \\
  & \hspace{18mm} + (\mathrm{SL}\ (SCOPE_P\ c_{cat}\ (\lambda y.\ \dforall
  x.\ (\eta\ (\obj{man}\ x \land \obj{know}\ x\ y)) \dimp (k\ x))))\ \eta \\
\rightarrow^*\ & SCOPE\ (\lambda k.\ (\mathrm{SL}\ (\dforall x.\
  \eta\ (\obj{man}\ x \land (\exists y.\ \obj{cat}\ y \land
  \obj{know}\ x\ y)) \dimp (k\ x))) \\
  & \hspace{18mm} + (c_{cat}\ (\lambda y.\ (\mathrm{SL}\ (\dforall
  x.\ (\eta\ (\obj{man}\ x \land \obj{know}\ x\ y)) \dimp (k\ x))))) \\
  & \hspace{18mm} + (SCOPE_P\ c_{cat}\ (\lambda y.\ \mathrm{SL}\ (\dforall
  x.\ (\eta\ (\obj{man}\ x \land \obj{know}\ x\ y)) \dimp (k\ x)))))\ \eta \\
\rightarrow^*\ & SCOPE\ (\lambda k.\ (\mathrm{SL}\ (\dforall x.\
  \eta\ (\obj{man}\ x \land (\exists y.\ \obj{cat}\ y \land
  \obj{know}\ x\ y)) \dimp (k\ x))) \\
  & \hspace{18mm} + (\mathrm{SL}\ (\dexists y.\ (\eta\ (\obj{cat}\ y)) \dand (\mathrm{SL}\ \dforall
  x.\ (\eta\ (\obj{man}\ x \land \obj{know}\ x\ y)) \dimp (k\ x)))) \\
  & \hspace{18mm} + (SCOPE_P\ c_{cat}\ (\lambda y.\ \mathrm{SL}\ (\dforall
  x.\ (\eta\ (\obj{man}\ x \land \obj{know}\ x\ y)) \dimp (k\ x)))))\ \eta \\
\end{align*}

\begin{align*}
  & \sem{\abs{loves}\ (\abs{a}\ \abs{woman})\ (\abs{every}\ (\abs{who}\ (\abs{knows}\ (\abs{a}\ \abs{cat}))\ \abs{man}))} \\
  \rightarrow^*\ & \mathrm{SI}\ (SCOPE\ (\mathrm{SL} \circ c_{man})\ 
  (\lambda x.\ SCOPE_P\ (\mathrm{SL} \circ c_{woman})\
  (\lambda z.\ \eta\ (\obj{love}\ x\ z)))) \\
  \rightarrow^*\ & \mathrm{SL}\ (c_{man}\ 
  (\lambda x.\ \mathrm{SI}\ (SCOPE_P\ (\mathrm{SL} \circ c_{woman})\
  (\lambda z.\ \eta\ (\obj{love}\ x\ z))))) \\
  \rightarrow^*\ & \mathrm{SL}\ (c_{man}\ 
  (\lambda x.\ (\mathrm{SL}\ (c_{woman}\ (\lambda
  z.\ \mathrm{SI}\ (\eta\ (\obj{love}\ x\ z))))) \\
  & \hspace{20mm} + (SCOPE_P\ (\mathrm{SL} \circ c_{woman})\
  (\lambda z.\ \mathrm{SI}\ (\eta\ (\obj{love}\ x\ z)))))) \\
  \rightarrow^*\ & \mathrm{SL}\ (c_{man}\ 
  (\lambda x.\ (\mathrm{SL}\ (c_{woman}\ (\lambda
  z.\ \eta\ (\obj{love}\ x\ z)))) \\
  & \hspace{20mm} + (SCOPE_P\ (\mathrm{SL} \circ c_{woman})\
  (\lambda z.\ \eta\ (\obj{love}\ x\ z))))) \\
\end{align*}
